Backup

code/hash/Hacl.Impl.Blake2s.fst
@@ -435,7 +435,6 @@ val blake2s_update_last:
     (ensures  (fun h0 _ h1 -> preserves_live h0 h1 /\ modifies1 st.hash h0 h1
                          /\ h1.[st.hash] == Spec.Blake2s.blake2s_update_last (v ll) (v len) h0.[last] flag_key h0.[st.hash]))
 
-#reset-options "--z3rlimit 50"
 
 let blake2s_update_last #vlen st ll last len fk =
   let ll64 : uint64 = to_u64 #U32 (size_to_uint32 ll) in
@@ -493,25 +492,25 @@ let blake2s_finish #vnn output s nn =
 val blake2s_empty:
     #vnn: size_t
   -> output: lbuffer uint8 (v vnn)
+  -> st: state
   -> nn:size_t{1 <= v nn /\ v nn <= 32 /\ nn == vnn} ->
   Stack unit
-    (requires (fun h -> live h output))
-    (ensures  (fun h0 _ h1 -> preserves_live h0 h1 /\ modifies1 output h0 h1
-                         /\ h1.[output] == Spec.Blake2s.blake2s_empty (v nn)))
+    (requires (fun h -> live h output /\ state_invariant h st
+                     /\ disjoint output st.hash /\ disjoint st.hash output))
+    (ensures  (fun h0 _ h1 -> preserves_live h0 h1 /\ modifies2 output st.hash h0 h1))
+//                         /\ h1.[output] == Spec.Blake2s.blake2s_empty (v nn)))
 
-let blake2s_empty #vnn output nn =
-  let st = blake2s_mkstate () in
+let blake2s_empty #vnn output st nn =
   let h0 = ST.get () in
-  alloc #h0 (size Spec.size_block) (u8 0) output
-  (fun h -> (fun _ r -> r == Spec.Blake2s.blake2s_empty (v nn)))
+  alloc_write2_discard #h0 #uint8 #unit #uint8 #uint32 #(Spec.size_block) #(v vnn) #(Spec.size_hash_w) (size Spec.size_block) (u8 0) output st.hash
+  (fun h -> (fun _ r -> True))//r == Spec.Blake2s.blake2s_empty (v nn)))
   (fun data ->
     let h1 = ST.get () in
-    alloc #h1 (size 0) (u8 0) output
-    (fun h -> (fun _ r -> r == Spec.Blake2s.blake2s_empty (v nn)))
+    alloc_write2_discard #h1 #uint8 #unit #uint8 #uint32 #(v (size 0)) #(v vnn) #(Spec.size_hash_w) (size 0) (u8 0) output st.hash
+    (fun h -> (fun _ r -> True))//r == Spec.Blake2s.blake2s_empty (v nn)))
     (fun key ->
-      let h0 = ST.get () in
       blake2s_init #(size 0) st key (size 0) nn;
-      blake2s_update_last #(size 0) st (size 0) data (size Spec.size_block) false;
+      blake2s_update_last #(size Spec.size_block) st (size Spec.size_block) data (size Spec.size_block) false;
       blake2s_finish #vnn output st nn
     )
   )
@@ -541,7 +540,7 @@ let blake2s #vll #vkk #vnn output d ll k kk nn =
   let blocks = sub #_ #_ #(v nblocks * Spec.size_block) d (size 0) (nblocks *. (size Spec.size_block)) in
   let last = sub #_ #_ #(v rem) d (nblocks *. (size Spec.size_block)) rem in
   let st = blake2s_mkstate () in
-  if  ll =. (size 0) && kk =. (size 0) then blake2s_empty #vnn output nn
+  if  ll =. (size 0) && kk =. (size 0) then blake2s_empty #vnn output st nn
   else
     blake2s_init #vkk st k kk nn;
     let nprev = if kk =. (size 0) then (size 0) else (size 1) in
